src/coq/Semantics/LLVMEvents.v
@@ -15,7 +15,6 @@ From Coq Require Import
      String
      Setoid
      Morphisms
-     Omega
      Classes.RelationClasses.
 
 From ExtLib Require Import
@@ -124,7 +123,7 @@ Set Contextual Implicit.
   Definition print_msg (msg : string) : unit := tt.
 
   Definition raise {E} {A} `{FailureE -< E} (msg : string) : itree E A :=
-    v <- trigger (Throw _ (print_msg msg));; match v: void with end.
+    v <- trigger (Throw (print_msg msg));; match v: void with end.
 
   #[global] Instance RAISE_ERR_ITREE_FAILUREE {E : Type -> Type} `{FailureE -< E} : RAISE_ERROR (itree E) :=
   { raise_error := fun A e => raise e
@@ -187,9 +186,15 @@ Module Type LLVM_INTERACTIONS (ADDR : MemoryAddress.ADDRESS) (IP:MemoryAddress.I
    is intended to be a predicate over the set of dvalues _u_ can take such that
    if it is not satisfied, the only possible execution is to raise _UB_.
    *)
-  Variant PickE : Type -> Type :=
-  | pick_uvalue (Pre : Prop) (u:uvalue) : PickE dvalue.
-    
+  Variant PickE {X Y} {Post : X -> Y -> Prop} : Type -> Type :=
+    | pick (Pre : Prop) (x : X) : PickE ({y : Y | Post x y}).
+
+  Definition PickUvalueE := @PickE uvalue dvalue (fun _ _ => True).
+  
+  (* MOVE THIS *)
+  Class RAISE_PICK {X Y Post} (M : Type -> Type) : Type :=
+    { raise_pick : @PickE X Y Post ~> M }.
+
   (* The signatures for computations that we will use during the successive stages of the interpretation of LLVM programs *)
   (* TODO: The events and handlers are parameterized by the types of key and value.
      It's weird for it to be the case if the events are concretely instantiated right here.
@@ -199,9 +204,9 @@ Module Type LLVM_INTERACTIONS (ADDR : MemoryAddress.ADDRESS) (IP:MemoryAddress.I
   Definition LLVMEnvE := (LocalE raw_id uvalue).
   Definition LLVMStackE := (StackE raw_id uvalue).
 
-  Definition conv_E := MemoryE +' PickE +' OOME +' UBE +' DebugE +' FailureE.
+  Definition conv_E := MemoryE +' PickUvalueE +' OOME +' UBE +' DebugE +' FailureE.
   Definition lookup_E := LLVMGEnvE +' LLVMEnvE.
-  Definition exp_E := LLVMGEnvE +' LLVMEnvE +' MemoryE +' PickE +' OOME +' UBE +' DebugE +' FailureE.
+  Definition exp_E := LLVMGEnvE +' LLVMEnvE +' MemoryE +' PickUvalueE +' OOME +' UBE +' DebugE +' FailureE.
 
   Definition LU_to_exp : lookup_E ~> exp_E :=
     fun T e =>
@@ -218,7 +223,7 @@ Module Type LLVM_INTERACTIONS (ADDR : MemoryAddress.ADDRESS) (IP:MemoryAddress.I
     fun T e => inr1 (inr1 e).
 
   (* Core effects. *)
-  Definition L0' := CallE +' ExternalCallE +' IntrinsicE +' LLVMGEnvE +' (LLVMEnvE +' LLVMStackE) +' MemoryE +' PickE +' OOME +' UBE +' DebugE +' FailureE.
+  Definition L0' := CallE +' ExternalCallE +' IntrinsicE +' LLVMGEnvE +' (LLVMEnvE +' LLVMStackE) +' MemoryE +' PickUvalueE +' OOME +' UBE +' DebugE +' FailureE.
 
   Definition instr_to_L0' : instr_E ~> L0' :=
     fun T e =>
@@ -248,7 +253,7 @@ Module Type LLVM_INTERACTIONS (ADDR : MemoryAddress.ADDRESS) (IP:MemoryAddress.I
       | inr1 (inr1 x) => inr1 (inr1 (inr1 (inr1 (inl1 x))))
       end.
 
-  Definition L0 := ExternalCallE +' IntrinsicE +' LLVMGEnvE +' (LLVMEnvE +' LLVMStackE) +' MemoryE +' PickE +' OOME +' UBE +' DebugE +' FailureE.
+  Definition L0 := ExternalCallE +' IntrinsicE +' LLVMGEnvE +' (LLVMEnvE +' LLVMStackE) +' MemoryE +' PickUvalueE +' OOME +' UBE +' DebugE +' FailureE.
 
   Definition exp_to_L0 : exp_E ~> L0 :=
     fun T e =>
@@ -259,15 +264,15 @@ Module Type LLVM_INTERACTIONS (ADDR : MemoryAddress.ADDRESS) (IP:MemoryAddress.I
       end.
 
   (* For multiple CFG, after interpreting [GlobalE] *)
-  Definition L1 := ExternalCallE +' IntrinsicE +' (LLVMEnvE +' LLVMStackE) +' MemoryE +' PickE +' OOME +' UBE +' DebugE +' FailureE.
+  Definition L1 := ExternalCallE +' IntrinsicE +' (LLVMEnvE +' LLVMStackE) +' MemoryE +' PickUvalueE +' OOME +' UBE +' DebugE +' FailureE.
 
   (* For multiple CFG, after interpreting [LocalE] *)
-  Definition L2 := ExternalCallE +' IntrinsicE +' MemoryE +' PickE +' OOME +' UBE +' DebugE +' FailureE.
+  Definition L2 := ExternalCallE +' IntrinsicE +' MemoryE +' PickUvalueE +' OOME +' UBE +' DebugE +' FailureE.
 
   (* For multiple CFG, after interpreting [LocalE] and [MemoryE] and [IntrinsicE] that are memory intrinsics *)
-  Definition L3 := ExternalCallE +' PickE +' OOME +' UBE +' DebugE +' FailureE.
+  Definition L3 := ExternalCallE +' PickUvalueE +' OOME +' UBE +' DebugE +' FailureE.
 
-  (* For multiple CFG, after interpreting [LocalE] and [MemoryE] and [IntrinsicE] that are memory intrinsics and [PickE]*)
+  (* For multiple CFG, after interpreting [LocalE] and [MemoryE] and [IntrinsicE] that are memory intrinsics and [PickUvalueE]*)
   Definition L4 := ExternalCallE +' OOME +' UBE +' DebugE +' FailureE.
 
   Definition L5 := ExternalCallE +' OOME +' DebugE +' FailureE.
